theories/Interp/TranslateFacts.v
@@ -60,31 +60,13 @@ Qed.
 Global Instance translate_Proper :
   Proper (eq_itree (@eq R) ==> eq_itree eq) (translate h).
 Proof.
-  repeat red.
-  intros x y H.
-  uinit.
-  revert x y H.
   ucofix CIH.
   intros x y H.
   rewrite itree_eta.
-  rewrite (itree_eta (translate h y)).
-  repeat rewrite unfold_translate. unfold translateF.
-  rewrite (itree_eta x) in H.
-  rewrite (itree_eta y) in H.
-  destruct (observe x); destruct (observe y); pinversion H; subst; cbn.
-  - ufinal. apply Reflexive_eq_itree. (* SAZ: typeclass resolution not working *)
-  - ufinal. pfold. constructor.  right. apply CIH. eauto.
-  - ufinal. pfold.
-    repeat (match goal with
-          | [ H : _ |- _ ] => apply inj_pair2 in H
-            end). subst.
-    constructor.
-    inversion H.
-    repeat (match goal with
-          | [ H : _ |- _ ] => apply inj_pair2 in H
-            end). subst.
-    right. apply CIH.
-    eapply transitivity. pclearbot. apply REL0. reflexivity.
+  rewrite (itree_eta (translate h y)), !unfold_translate, <-!itree_eta.
+  rewrite (itree_eta x), (itree_eta y) in H.
+  uunfold H. genobs_clear x ox. genobs_clear y oy. repeat red in H.
+  destruct ox, oy; dependent destruction H; constructor; eauto with paco.
 Qed.
 
 Global Instance translateF_Proper :
@@ -103,16 +85,14 @@ Lemma translate_bind : forall {E F R S} (h : E ~> F) (t : itree E S) (k : S -> i
     translate h (x <- t ;; k x) ≅ (x <- (translate h t) ;; translate h (k x)).
 Proof.
   intros E F R S h t k.
-  uinit.
   revert S t k.
   ucofix CIH.
   intros s t k.
   rewrite !unfold_translate, !unfold_bind.
   genobs_clear t ot. destruct ot; cbn.
-  - rewrite unfold_translate.
-    ufinal. apply Reflexive_eq_itree.
-  - econstructor. ufinal. right. apply CIH.
-  - econstructor. intros.  ufinal. right. apply CIH.
+  - rewrite unfold_translate. apply reflexivity.
+  - econstructor. ubase. apply CIH.
+  - econstructor. intros. ubase. apply CIH.
 Qed.
 
 (* categorical properties --------------------------------------------------- *)
@@ -120,7 +100,6 @@ Qed.
 Lemma translate_id : forall E R (t : itree E R), translate (id_ _) t ≅ t.
 Proof.
   intros E R t.
-  uinit.
   revert t.
   ucofix CIH.
   intros t.
@@ -129,9 +108,9 @@ Proof.
   rewrite unfold_translate.
   unfold translateF.
   destruct (observe t); cbn.
-  - ufinal. apply Reflexive_eq_itree.
-  - econstructor. ufinal. right.  apply CIH.
-  - econstructor. intros. ufinal. right.  apply CIH.
+  - apply reflexivity.
+  - econstructor. ubase. apply CIH.
+  - econstructor. intros. ubase. apply CIH.
 Qed.
 
 Import CatNotations.
@@ -140,15 +119,14 @@ Lemma translate_cmpE : forall E F G R (g : F ~> G) (f : E ~> F) (t : itree E R),
     translate (f >>> g)%cat t ≅ translate g (translate f t).
 Proof.
   intros E F G R g f t.
-  uinit.
   revert t.
   ucofix CIH.
   intros t.
   rewrite !unfold_translate.
   genobs_clear t ot. destruct ot; cbn.
-  - ufinal. apply reflexivity.
-  - econstructor. ufinal. right.  apply CIH.
-  - econstructor. intros. ufinal. right.  apply CIH.
+  - apply reflexivity.
+  - econstructor. ubase. apply CIH.
+  - econstructor. intros. ubase. apply CIH.
 Qed.
 
 (* SAZ: TODO - it would be good to allow for rewriting of event morphisms under translate:
